simplify verifier

Veritas.Verifier.Correctness.fst
@@ -13,28 +13,56 @@ open Veritas.Verifier
 //Allow the solver to invert inductive definitions at most once (ifuel)
 #push-options "--max_fuel 1 --max_ifuel 1 --initial_fuel 1 --initial_ifuel 1"
 
-(* type of thread ids *)
-type tid (p:pos) = id:nat{id < p}
+(* 
+ * an indexed vlog attaches an nat index to a vlog 
+ * indicating the id of the verifier thread processing
+ * the log 
+ *)
+type tid_vlog = nat * vlog
+
+(* thread id of the indexed vlog *)
+let tid (il: tid_vlog) = fst il
+
+(* vlog of an indexed vlog *)
+let vlog_of (il: tid_vlog) = snd il
+
+(* length of the vlog portion *)
+let tv_length (tl: tid_vlog) = 
+  length (vlog_of tl)
+
+(* element at the i'th position of the vlog *)
+let tv_index (tl: tid_vlog) (i:nat{i < tv_length tl}) = 
+  index (vlog_of tl) i
+
+(* append an element at the end of the vlog *)
+let tv_append1 (tl: tid_vlog) (e: vlog_entry): Tot tid_vlog = 
+  (tid tl), (append1 (vlog_of tl) e)
+
+(* prefix of a tid_vlog: apply prefix on the 
+ * vlog component *)
+let tv_prefix (tl: tid_vlog) (i:nat{i <= tv_length tl}): Tot tid_vlog = 
+  (tid tl), (prefix (vlog_of tl) i)
 
 (* does the log leave the verifier thread in a valid state *)
-let t_verifiable (#p:pos) (id: tid p)  (l: vlog #p) = Valid? (t_verify id l)
+let t_verifiable (il: tid_vlog) = 
+  Valid? (t_verify (tid il) (vlog_of il))
 
-(* refinement types of valid thread-level logs *)
-type t_verifiable_log (#p:pos) (id: tid p) = l:(vlog #p){t_verifiable id l}
+(* refinement types of valid verifier logs *)
+type t_verifiable_log = il: tid_vlog {t_verifiable il}
 
 (* Full collection of verifier logs one per thread *)
-type g_vlog (#p:pos) = ss:seq (vlog #p){length ss <= p}
+type g_vlog = seq vlog
 
 (* globally verifiable logs *)
-type g_verifiable (#p:pos) (lg:g_vlog #p) = 
-  forall (i:nat{i < length lg}). {:pattern t_verifiable #p i (index lg i)} 
-  t_verifiable i (index lg i)
+type g_verifiable (lg:g_vlog) = 
+  forall (i:nat{i < length lg}). {:pattern t_verifiable (i, (index lg i))}
+  t_verifiable (i, (index lg i))
 
 (* Refinement type of logs that are verifiable *)
-type g_verifiable_log (#p:pos) = l:g_vlog{g_verifiable #p l}
+type g_verifiable_log = l:g_vlog{g_verifiable l}
 
 (* aggregate hadd over all verifier threads *)
-let rec g_hadd (#p:pos) (lg:g_verifiable_log #p) (e:nat)
+let rec g_hadd (lg:g_verifiable_log) (e:nat)
   : Tot ms_hash_value (decreases (length lg)) = 
   let n = length lg in
   if n = 0 then empty_hash_value
@@ -43,12 +71,12 @@ let rec g_hadd (#p:pos) (lg:g_verifiable_log #p) (e:nat)
     let hv' = g_hadd lg' e in
     let l = index lg (n - 1) in
     // TODO: how to remove this side-effect assert?
-    assert(t_verifiable (n - 1) l);
+    assert(t_verifiable ((n - 1), l));
     let h = thread_hadd (t_verify (n-1) l) e in
     ms_hashfn_agg hv' h  
 
 (* aggregate hadd over all verifier threads *)
-let rec g_hevict (#p:pos) (lg:g_verifiable_log #p) (e:nat)
+let rec g_hevict (lg:g_verifiable_log) (e:nat)
   : Tot ms_hash_value (decreases (length lg)) = 
   let n = length lg in
   if n = 0 then empty_hash_value
@@ -57,69 +85,85 @@ let rec g_hevict (#p:pos) (lg:g_verifiable_log #p) (e:nat)
     let hv' = g_hevict lg' e in
     let l = index lg (n - 1) in
     // TODO: how to remove this side-effect assert?
-    assert(t_verifiable  (n - 1) l);
+    assert(t_verifiable  ((n - 1), l));
     let h = thread_hevict (t_verify (n- 1) l) e in
     ms_hashfn_agg hv' h  
 
 (* verifiable logs where the first e epochs have identical hadd and hevict *)
-let ep_verifieable_log (#p:pos) (ep:pos) = 
-  l:(g_verifiable_log #p){forall (e:nat{e < ep}). g_hadd l e = g_hevict l e}
+type ep_verifiable_log (ep:pos) = 
+  l:(g_verifiable_log){forall (e:nat{e < ep}). g_hadd l e = g_hevict l e}
 
-(* the clock of a verifier thread after processing a verfiable log *)
-let clock_after (#p:pos) (#id:tid p) (l:t_verifiable_log id) = 
-  let vs = t_verify id l in
+(* the clock of a verifier thread after processing a verifiable log *)
+let clock_after (il:t_verifiable_log) = 
+  let vs = t_verify (tid il) (vlog_of il) in
   Valid?.clk vs
 
 let rec lemma_verifiable_implies_prefix_verifiable
-  (#p:pos) (id:tid p) (l:t_verifiable_log id) (i:nat{i <= length l}):
+  (tl:t_verifiable_log) (i:nat{i <= tv_length tl}):
   Lemma (requires (True))
-        (ensures (t_verifiable id (prefix l i)))
-        (decreases (length l)) 
-        =
-  let n = length l in
+        (ensures (t_verifiable (tv_prefix tl i)))
+        (decreases (tv_length tl)) 
+        [SMTPat (tv_prefix tl i)]
+        =    
+  let n = tv_length tl in
   if n = 0 then ()
   else if i = n then ()
   else
-    lemma_verifiable_implies_prefix_verifiable id (prefix l (n - 1)) i
-
-(* TODO: Adding SMTPat (prefix l i) does not work in the lemma_above *)
-let t_vprefix (#p:pos) (#id:tid p) (l:t_verifiable_log id) (i:nat{i <= length l}): 
-  l':(t_verifiable_log id){l' = prefix l i} = 
-  let l' = prefix l i in
-  lemma_verifiable_implies_prefix_verifiable id l i;
-  l'
+    lemma_verifiable_implies_prefix_verifiable (tv_prefix tl (n - 1)) i
 
 (* the clock of a verifier is monotonic *)
-let rec lemma_clock_monotonic (#p:pos) (#id:tid p) (l:t_verifiable_log id)
-                          (i:nat{i <= length l}):
+let rec lemma_clock_monotonic (tl:t_verifiable_log) (i:nat{i <= tv_length tl}):
   Lemma (requires(True))
-        (ensures (clock_after (t_vprefix l i) `ts_leq` clock_after l)) 
-  (decreases (length l))        
+        (ensures (clock_after (tv_prefix tl i) `ts_leq` clock_after tl)) 
+  (decreases (tv_length tl))        
         = 
-  let n = length l in
+  let n = tv_length tl in
   if n = 0 then ()
   else if i = n then ()
   else
-    let l' = t_vprefix l (n - 1) in
-    lemma_clock_monotonic l' i
+    let tl' = tv_prefix tl (n - 1) in
+    lemma_clock_monotonic tl' i
 
-type clocked_vlog_entry (#p:nat) = vlog_entry #p * timestamp
+type clocked_vlog_entry = vlog_entry * timestamp
 
-type clocked_vlog (#p:nat) = seq (clocked_vlog_entry #p)
+type clocked_vlog = seq (clocked_vlog_entry)
 
-let rec attach_clock (#p:pos) (id:tid p) (l:t_verifiable_log id): 
-  Tot (clocked_vlog #p) 
-  (decreases (length l)) = 
-  let n = length l in
+(* construct an augmented vlog with the clock
+ * attached to every vlog entry *)
+let rec attach_clock (tl:t_verifiable_log): 
+  Tot (clocked_vlog) 
+  (decreases (tv_length tl)) = 
+  let n = tv_length tl in
   if n = 0 then empty 
   else 
-    let l' = t_vprefix l (n - 1) in
-    let cl' = attach_clock id l' in
-    let t = clock_after l in
-    let e = index l (n - 1) in
-    append cl' (create 1 (e, t))
+    let tl' = tv_prefix tl (n - 1) in
+    let cl' = attach_clock tl' in
+    let t = clock_after tl in
+    let e = tv_index tl (n - 1) in
+    append1 cl' (e, t)
 
-(* is s' a prefix of s *)
-let is_prefix (#a:eqtype) (s':seq a) (s:seq a) = 
-  length s' <= length s && prefix s (length s') = s'
+(* the state operations of a vlog *)
+let is_state_op (e: vlog_entry) = 
+  match e with
+  | Get k v -> true
+  | Put k v -> true 
+  | _ -> false
 
+(* map vlog entry to state op *)
+let to_state_op (e:vlog_entry {is_state_op e}) = 
+  match e with
+  | Get k v -> Veritas.State.Get k v
+  | Put k v -> Veritas.State.Put k v
+
+(* filter out the state ops of vlog *)
+let to_state_op_vlog (l: vlog) = 
+  map to_state_op (filter_refine is_state_op l)
+
+(* state ops of all vlogs of all verifier threads *)
+let to_state_op_gvlog (gl: g_vlog) = 
+  map to_state_op_vlog gl
+
+
+let lemma_verifier_correct (ep:pos) (l:(ep_verifiable_log ep)):
+  Lemma (requires (True))
+        (ensures (False)) = admit()
